sepcomp-reserved/forward_simulations_lemmas.v
@@ -50,7 +50,7 @@ Section Sim_EQ_SIMU_DIAGRAMS.
     (at_external Sem2 st2 = Some (e, ef_sig, args) /\
      Forall2 Val.has_type args (sig_args ef_sig)).
 
-Hypothesis eq_after_external:
+  Hypothesis eq_after_external:
    forall (d : C1) (st1 : core_data) (st2 : C2) (ret : val) 
           (e : external_function) (args : list val) (ef_sig : signature),
     (d = st1 /\ match_cores d st1 st2) ->
@@ -135,8 +135,8 @@ End Sim_EQ_SIMU_DIAGRAMS.
 
 Section Sim_EXT_SIMU_DIAGRAMS.
   Context {G1 C1 D1 G2 C2 D2:Type}
-          {Sem1 : RelyGuaranteeSemantics G1 C1 D1}
-          {Sem2 : RelyGuaranteeSemantics G2 C2 D2}
+          {Sem1 : EffectfulSemantics G1 C1 D1}
+          {Sem2 : EffectfulSemantics G2 C2 D2}
 
           {ge1:G1}
           {ge2:G2}
@@ -144,12 +144,21 @@ Section Sim_EXT_SIMU_DIAGRAMS.
 
   Let core_data := C1.
 
-  Variable match_states: core_data -> reserve_map -> C1 -> mem -> C2 -> mem -> Prop.
+  Variable match_states: core_data -> reserve -> C1 -> mem -> C2 -> mem -> Prop.
 
-  Variable reserve_valid: 
+  Variable match_memwd:
+    forall cd r c1 m1 c2 m2, 
+      match_states cd r c1 m1 c2 m2 -> mem_wd m1 /\ mem_wd m2.
+
+  Variable match_valid:
     forall cd r c1 m1 c2 m2,
       match_states cd r c1 m1 c2 m2 -> 
-      reserve_map_valid r m1 /\ reserve_map_valid r m2.
+      forall b, Mem.valid_block m1 b <-> Mem.valid_block m2 b.
+
+  Variable reserved_locs_valid: 
+    forall cd r c1 m1 c2 m2,
+      match_states cd r c1 m1 c2 m2 -> 
+      reserve_valid r m1 /\ reserve_valid r m2.
 
   Hypothesis match_initial_cores: forall v1 v2 sig,
       In (v1,v2,sig) entry_points ->
@@ -157,8 +166,8 @@ Section Sim_EXT_SIMU_DIAGRAMS.
           Forall2 Val.lessdef vals vals' ->
           Forall2 (Val.has_type) vals' (sig_args sig) ->
           Mem.extends m1 m2 ->
-          reserve_map_valid r m1 -> 
-          reserve_map_valid r m2 -> 
+          reserve_valid r m1 -> reserve_valid r m2 -> 
+          mem_wd m1 -> mem_wd m2 ->
           exists c1, exists c2,
             make_initial_core Sem1 ge1 v1 vals = Some c1 /\
             make_initial_core Sem2 ge2 v2 vals' = Some c2 /\
@@ -175,12 +184,14 @@ Section Sim_EXT_SIMU_DIAGRAMS.
   Hypothesis ext_at_external: 
         forall d r st1 m1 st2 m2 e vals1 sig,
           (d = st1 /\ match_states d r st1 m1 st2 m2) ->
-         at_external Sem1 st1 = Some (e, sig, vals1) ->
-         exists vals2,
+        at_external Sem1 st1 = Some (e,sig,vals1) ->
+        (forall v1, In v1 vals1 -> val_valid v1 m1) -> 
+        exists vals2,
           Mem.extends m1 m2 /\
           Forall2 Val.lessdef vals1 vals2 /\
           Forall2 (Val.has_type) vals2 (sig_args sig) /\
-          at_external Sem2 st2 = Some (e,sig,vals2).
+          at_external Sem2 st2 = Some (e,sig,vals2) /\
+          (forall v2, In v2 vals2 -> val_valid v2 m2).
 
   Hypothesis ext_after_external:
       forall d r st1 st2 m1 m2 e vals1 vals2 ret1 ret2 r' m1' m2' ef_sig,
@@ -193,16 +204,16 @@ Section Sim_EXT_SIMU_DIAGRAMS.
         mem_forward m1 m1' ->
         mem_forward m2 m2' ->
 
-        mem_unchanged_on (fun b ofs => ~r b ofs /\ owned Sem2 st2 b ofs) m2 m2' -> 
+        rely Sem2 r st2 m2 m2' -> 
         Val.lessdef ret1 ret2 ->
         Mem.extends m1' m2' ->
 
         Val.has_type ret2 (proj_sig_res ef_sig) -> 
 
-        reserve_map_incr r r' -> 
-        reserve_map_separated r r' inject_id m1 m2 -> 
-
-        Val.has_type ret2 (proj_sig_res ef_sig) ->
+        reserve_incr r r' -> 
+        reserve_separated r r' inject_id m1 m2 -> 
+        mem_wd m1' -> mem_wd m2' -> 
+        val_valid ret1 m1' -> val_valid ret2 m2' ->
 
         exists st1', exists st2', exists d',
           after_external Sem1 (Some ret1) st1 = Some st1' /\
@@ -215,12 +226,14 @@ Hypothesis order_wf: well_founded order.
 
 Hypothesis ext_simulation:
   forall r c1 m1 c1' m1',  corestep Sem1 ge1 c1 m1 c1' m1' ->
-    forall c2 m2, match_states c1 r c1 m1 c2 m2 ->
+    forall c2 m2, 
+      match_states c1 r c1 m1 c2 m2 ->
+      guarantee Sem1 r c1' m1' -> 
       exists c2', exists r', exists m2', 
-        reserve_map_incr r r' /\
-        reserve_map_separated r r' inject_id m1 m2 /\
+        reserve_incr r r' /\
+        reserve_separated r r' inject_id m1 m2 /\
         match_states c1' r' c1' m1' c2' m2' /\
-        mem_unchanged_on (guarantee_right Sem1 inject_id r c1) m2 m2' /\
+        guarantee Sem2 r c2' m2' /\
         (corestep_plus Sem2 ge2  c2 m2 c2' m2' \/ 
           (corestep_star Sem2 ge2 c2 m2 c2' m2' /\ order c1' c1)).
 
@@ -233,29 +246,28 @@ Proof.
   apply order_wf.
   intros; destruct H; subst.
   split; auto.
-  exploit reserve_valid; eauto.
+  exploit match_memwd; eauto.
   solve[intros [? ?]; auto].
-  exploit reserve_valid; eauto.
-  intros [? ?].
-  unfold reserve_map_valid_right.
-  intros b b2 delta ofs H2.
-  unfold inject_id; intros H3.
-  inv H3.
-  unfold reserve_map_valid in H1.
-  solve[apply (H1 b2 ofs); auto].
+  exploit match_memwd; eauto.
+  solve[intros [? ?]; auto].
+  intros; destruct H.
+  solve[exploit match_valid; eauto].
+  intros; destruct H.
+  exploit reserved_locs_valid; eauto.
+  intros [? X]; split; auto.
+  unfold reserve_valid'; hnf.
+  intros.
+  unfold inject_id in H3.
+  solve[inv H3; eapply X; eauto].
   intros; destruct H0 as [? ?]; subst.
   exploit ext_simulation; eauto.  
   intros [c2' [r' [m2' [? [? [? [? Step]]]]]]].
-  exists c2'. exists r'.  exists m2'. exists st1'. 
+  exists c2'. exists r'. exists m2'. exists st1'. 
   solve[split; auto].
   intros.
   exploit match_initial_cores; eauto.
-  unfold reserve_map_valid_right, inject_id in H4.
-  intros b ofs H5.
-  specialize (H4 b b 0 ofs).
-  solve[apply H4; auto].
-  intros [c1' [c2' [? [? ?]]]].
-  solve[do 3 eexists; eauto].
+  intros [c1 [c2 [? [? ?]]]].
+  solve[exists c1, c1, c2; split; auto].
   intros.
   destruct H as [Heq ?]; subst.
   exploit ext_safely_halted; eauto.
@@ -271,15 +283,16 @@ Section EXT_SIMULATION_STAR.
   Variable measure: C1 -> nat.
   
   Hypothesis ext_star_simulation:
-    forall (c1 : C1) r (m1 : mem) (c1' : C1) (m1' : mem),
+    forall (c1 : C1) (r: reserve) (m1 : mem) (c1' : C1) (m1' : mem),
       corestep Sem1 ge1 c1 m1 c1' m1' ->
       forall (c2 : C2) (m2 : mem),
+        guarantee Sem1 r c1' m1' -> 
         match_states c1 r c1 m1 c2 m2 ->
         exists c2' r' m2', 
-          reserve_map_incr r r' /\
-          reserve_map_separated r r' inject_id m1 m2 /\
+          reserve_incr r r' /\
+          reserve_separated r r' inject_id m1 m2 /\
           match_states c1' r' c1' m1' c2' m2' /\
-          mem_unchanged_on (guarantee_right Sem1 inject_id r c1) m2 m2' /\
+          guarantee Sem2 r c2' m2' /\
           (corestep_plus Sem2 ge2 c2 m2 c2' m2' \/ 
            corestep_star Sem2 ge2 c2 m2 c2' m2' /\ ltof C1 measure c1' c1).
 
@@ -297,12 +310,14 @@ Section EXT_SIMULATION_PLUS.
   Variable measure: C1 -> nat. 
   Hypothesis ext_plus_simulation:
     forall c1 r m1 c1' m1', corestep Sem1 ge1 c1 m1 c1' m1'  -> 
-    forall c2 m2, match_states c1 r c1 m1 c2 m2 ->
+    forall c2 m2, 
+      match_states c1 r c1 m1 c2 m2 ->
+      guarantee Sem1 r c1' m1' -> 
       exists c2' r' m2',
-        reserve_map_incr r r' /\
-        reserve_map_separated r r' inject_id m1 m2 /\
+        reserve_incr r r' /\
+        reserve_separated r r' inject_id m1 m2 /\
         match_states c1' r' c1' m1' c2' m2' /\
-        mem_unchanged_on (guarantee_right Sem1 inject_id r c1) m2 m2' /\
+        guarantee Sem2 r c2' m2' /\
         corestep_plus Sem2 ge2 c2 m2 c2' m2'.
 
 Lemma ext_simulation_plus: 
@@ -320,8 +335,8 @@ End Sim_EXT_SIMU_DIAGRAMS.
 
 Section Sim_INJ_SIMU_DIAGRAMS.
   Context {F1 V1 C1 D1 G2 C2 D2:Type}
-          {Sem1 : RelyGuaranteeSemantics (Genv.t F1 V1) C1 D1}
-          {Sem2 : RelyGuaranteeSemantics G2 C2 D2}
+          {Sem1 : EffectfulSemantics (Genv.t F1 V1) C1 D1}
+          {Sem2 : EffectfulSemantics G2 C2 D2}
 
           {ge1: Genv.t F1 V1} 
           {ge2:G2}
@@ -329,44 +344,74 @@ Section Sim_INJ_SIMU_DIAGRAMS.
 
   Let core_data := C1.
 
-  Variable match_states: core_data -> reserve_map -> meminj -> C1 -> mem -> C2 -> mem -> Prop.
+  Variable match_states: core_data -> reserve -> meminj -> C1 -> mem -> C2 -> mem -> Prop.
 
-  Hypothesis reserve_valid: 
-    forall cd r j c1 m1 c2 m2,
-      match_states cd r j c1 m1 c2 m2 -> 
-      reserve_map_valid r m1 /\ reserve_map_valid_right r j m2.
+   Variable match_memwd : 
+     forall cd r j c1 m1 c2 m2, 
+       match_states cd r j c1 m1 c2 m2 -> mem_wd m1 /\ mem_wd m2.
+
+   Variable reserved_locs_valid :
+      forall cd r j c1 m1 c2 m2,
+        match_states cd r j c1 m1 c2 m2 -> 
+        reserve_valid r m1 /\ reserve_valid' r j m2.
+
+   Variable effects_valid : forall cd r j c1 m1 c2 m2,
+     match_states cd r j c1 m1 c2 m2 -> 
+     effects_valid Sem1 c1 m1 /\ effects_valid Sem2 c2 m2.
+
+   Variable allocs_only_shrink: forall cd r j st1 m1 st2 m2, 
+     match_states cd r j st1 m1 st2 m2 ->
+     forall b2 ofs2, effects Sem2 st2 AllocEffect b2 ofs2 ->
+       forall b1 delta, 
+         j b1 = Some (b2, delta) ->
+         effects Sem1 st1 AllocEffect b1 (ofs2 - delta).
+
+   Variable match_antimono : 
+     forall d r0 r j st m st' m',
+       match_states d r j st m st' m' ->
+       reserve_incr r0 r -> 
+       match_states d r0 j st m st' m'.
+       
+   Variable match_validblocks : 
+     forall d r j c1 m1 c2 m2, 
+       match_states d r j c1 m1 c2 m2 -> 
+       forall b1 b2 ofs, j b1 = Some(b2,ofs) -> 
+         Mem.valid_block m1 b1 /\ Mem.valid_block m2 b2.
 
   Hypothesis match_initial_cores: forall v1 v2 sig,
-        In (v1,v2,sig) entry_points -> 
-       forall vals1 c1 r m1 j vals2 m2,
+       In (v1,v2,sig) entry_points -> 
+       forall vals1 c1 m1 j vals2 r m2,
           make_initial_core Sem1 ge1 v1 vals1 = Some c1 ->
           Mem.inject j m1 m2 -> 
+          mem_wd m1 -> mem_wd m2 ->
           Forall2 (val_inject j) vals1 vals2 ->
           Forall2 (Val.has_type) vals2 (sig_args sig) ->
-          reserve_map_valid r m1 -> 
-          reserve_map_valid_right r j m2 -> 
-          exists c2, 
+          reserve_valid r m1 -> 
+          reserve_valid' r j m2 -> 
+          exists c2,
             make_initial_core Sem2 ge2 v2 vals2 = Some c2 /\
-            match_states c1 r j c1 m1 c2 m2. 
+            match_states c1 r j c1 m1 c2 m2.
 
   Hypothesis inj_safely_halted:forall cd r j c1 m1 c2 m2 v1 rty,
       match_states cd r j c1 m1 c2 m2 ->
       safely_halted Sem1 c1 = Some v1 ->
       Val.has_type v1 rty -> 
-      exists v2, val_inject j v1 v2 /\ 
-        safely_halted Sem2 c2 = Some v2 /\
-        Val.has_type v2 rty /\
-        Mem.inject j m1 m2.
+      exists v2, val_inject j v1 v2 /\
+          safely_halted Sem2 c2 = Some v2 /\
+          Val.has_type v2 rty /\
+          Mem.inject j m1 m2.
 
   Hypothesis inj_at_external: 
       forall d j st1 r m1 st2 m2 e vals1 sig,
         d = st1 /\ match_states d r j st1 m1 st2 m2 ->
         at_external Sem1 st1 = Some (e,sig,vals1) ->
+        (forall v1, In v1 vals1 -> val_valid v1 m1) ->
         Mem.inject j m1 m2 /\
         meminj_preserves_globals ge1 j /\ 
         exists vals2, Forall2 (val_inject j) vals1 vals2 /\
                       Forall2 (Val.has_type) vals2 (sig_args (ef_sig e)) /\
-                      at_external Sem2 st2 = Some (e,sig,vals2).
+                      at_external Sem2 st2 = Some (e,sig,vals2) /\
+                      (forall v2, In v2 vals2 -> val_valid v2 m2).
 
   Hypothesis inj_after_external:
       forall d r r' j j' st1 st2 m1 e vals1 ret1 m1' m2 m2' ret2 sig,
@@ -377,19 +422,21 @@ Section Sim_INJ_SIMU_DIAGRAMS.
         inject_incr j j' ->
         inject_separated j j' m1 m2 ->
 
-        reserve_map_incr r r' -> 
-        reserve_map_separated r r' j' m1 m2 -> 
+        reserve_incr r r' -> 
+        reserve_separated r r' j' m1 m2 -> 
 
         Mem.inject j' m1' m2' ->
+        mem_wd m1' -> mem_wd m2' ->
         val_inject_opt j' ret1 ret2 ->
 
         mem_forward m1 m1'  -> 
         mem_forward m2 m2' -> 
-        mem_unchanged_on (rely_left Sem1 r st1) m1 m1' -> 
-        mem_unchanged_on (rely_right Sem1 j r st1) m2 m2' -> 
+        rely Sem1 r st1 m1 m1' -> 
 
-        val_has_type_opt' ret1 (proj_sig_res (ef_sig e)) ->
-        val_has_type_opt' ret2 (proj_sig_res (ef_sig e)) ->
+        rely' Sem2 j r st2 m2 m2' -> 
+
+        val_has_type_opt' ret1 (proj_sig_res (ef_sig e)) -> 
+        val_has_type_opt' ret2 (proj_sig_res (ef_sig e)) -> 
 
         exists st1', exists st2', exists d',
           after_external Sem1 ret1 st1 = Some st1' /\
@@ -401,18 +448,20 @@ Variable order: C1 -> C1 -> Prop.
 Hypothesis order_wf: well_founded order.
 
   Hypothesis inj_simulation:
-     forall c1 m1 c1' m1',  corestep Sem1 ge1 c1 m1 c1' m1' ->
-     forall j r c2 m2, match_states c1 r j c1 m1 c2 m2 ->
-      exists c2', exists m2', exists r', exists j', 
-        inject_incr j j' /\
-        inject_separated j j' m1 m2 /\
-        match_states c1' r' j' c1' m1' c2' m2' /\
-        reserve_map_incr r r' /\
-        reserve_map_separated r r' j' m1 m2 /\ 
-        mem_unchanged_on (guarantee_left Sem1 r c1) m1 m1' /\
-        mem_unchanged_on (guarantee_right Sem1 j r c1) m2 m2' /\
-        (corestep_plus Sem2 ge2  c2 m2 c2' m2' \/ 
-          (corestep_star Sem2 ge2 c2 m2 c2' m2' /\ order c1' c1)).
+    forall c1 m1 c1' m1', corestep Sem1 ge1 c1 m1 c1' m1' ->
+      forall j (r: reserve) c2 m2,
+        guarantee Sem1 r c1' m1' -> 
+        match_states c1 r j c1 m1 c2 m2 ->
+        exists c2', exists m2', exists r': reserve, exists j',
+          inject_incr j j' /\
+          inject_separated j j' m1 m2 /\
+          reserve_incr r r' /\
+          reserve_separated r r' j' m1 m2 /\ 
+          guarantee' Sem2 j r c2' m2' /\
+          match_states c1' r' j' c1' m1' c2' m2' /\
+          ((corestep_plus Sem2 ge2 c2 m2 c2' m2') \/
+            corestep_star Sem2 ge2 c2 m2 c2' m2' /\
+            order c1' c1).
 
 Lemma  inj_simulation_star_wf: 
   Forward_simulation_inj.Forward_simulation_inject _ _ Sem1 Sem2 ge1 ge2 entry_points.
@@ -422,10 +471,21 @@ Proof.
     (match_state := fun d r j c1 m1 c2 m2 => d = c1 /\ match_states d r j c1 m1 c2 m2).
   apply order_wf.
   intros. destruct H; subst.
-  solve[exploit reserve_valid; eauto].
-  intros. destruct H0; subst.
+  solve[exploit match_memwd; eauto].
+  intros; destruct H.
+  solve[exploit reserved_locs_valid; eauto].
+  intros. destruct H; subst.
+  solve[exploit effects_valid; eauto].
+  intros. destruct H; subst.
+  solve[exploit allocs_only_shrink; eauto].
+  intros. destruct H; subst.
+  split; auto.
+  solve[exploit match_antimono; eauto].
+  intros. destruct H; subst.
+  solve[exploit match_validblocks; eauto].
+  intros. destruct H1; subst.
   exploit inj_simulation; eauto.
-  intros [c2' [m2' [r' [j' [? [? [? [? [? [? [? ?]]]]]]]]]]].
+  intros [c2' [m2' [r' [j' [? [? [? [? [? [? ?]]]]]]]]]].
   exists c2'. exists m2'. exists st1'. exists r'. exists j'. 
   split; auto. split; auto. solve[split; auto].
   intros. exploit match_initial_cores; eauto. intros [c2 [? ?]].
@@ -434,7 +494,7 @@ Proof.
   solve[exploit inj_safely_halted; eauto].
   intros. destruct H. subst.
   solve[exploit inj_at_external; eauto].
-  intros. destruct H0; subst. 
+  intros. destruct H; subst. 
   exploit inj_after_external; eauto.
   intros [c1' [c2' [d' [? [? [? ?]]]]]]. subst.
   solve[exists c1', c1', c2'; split; auto].
@@ -446,31 +506,33 @@ Section INJ_SIMULATION_STAR.
   Variable measure: C1 -> nat.
   
   Hypothesis inj_star_simulation:
-    forall c1 m1 c1' m1', corestep Sem1 ge1 c1 m1 c1' m1'  -> 
-    forall c2 r m2 j, match_states c1 r j c1 m1 c2 m2 ->
-      (exists c2', exists m2', exists r', exists j', 
-        inject_incr j j' /\
-        inject_separated j j' m1 m2 /\ 
-        reserve_map_incr r r' /\
-        reserve_map_separated r r' j' m1 m2 /\ 
-        mem_unchanged_on (guarantee_left Sem1 r c1) m1 m1' /\
-        mem_unchanged_on (guarantee_right Sem1 j r c1) m2 m2' /\
-        match_states c1' r' j' c1' m1' c2' m2' /\
-        (corestep_plus Sem2 ge2 c2 m2 c2' m2' 
-          \/ ((measure c1' < measure c1)%nat /\ corestep_star Sem2 ge2 c2 m2 c2' m2'))).
-
+    forall c1 m1 c1' m1', 
+      corestep Sem1 ge1 c1 m1 c1' m1'  -> 
+      forall c2 (r: reserve) m2 j, 
+        guarantee Sem1 r c1' m1' -> 
+        match_states c1 r j c1 m1 c2 m2 ->
+        (exists c2', exists m2', exists r', exists j', 
+          inject_incr j j' /\
+          inject_separated j j' m1 m2 /\ 
+          reserve_incr r r' /\
+          reserve_separated r r' j' m1 m2 /\ 
+          guarantee' Sem2 j r c2' m2' /\
+          match_states c1' r' j' c1' m1' c2' m2' /\
+          (corestep_plus Sem2 ge2 c2 m2 c2' m2' 
+            \/ ((measure c1' < measure c1)%nat /\ corestep_star Sem2 ge2 c2 m2 c2' m2'))).
+  
 Lemma inj_simulation_star: 
   Forward_simulation_inj.Forward_simulation_inject _ _ Sem1 Sem2 ge1 ge2 entry_points.
 Proof.
   eapply inj_simulation_star_wf.
   apply  (well_founded_ltof _ measure).
   intros. exploit inj_star_simulation; eauto.
-  intros [c2' [m2' [r' [j' [? [? [? [? [? [? [? H8]]]]]]]]]]].
+  intros [c2' [m2' [r' [j' [? [? [? [? [? [? H8]]]]]]]]]].
   destruct H8.
-  exists c2', m2', r', j'; split; auto. split; auto. split; auto. solve[split; auto].
+  exists c2', m2', r', j'; split; auto. split; auto. split; auto. 
   destruct H8 as [? ?].
   exists c2', m2', r', j'; split; auto. split; auto. split; auto. 
-   split; auto. solve[split; auto].
+   split; auto. 
 Qed.
 
 End INJ_SIMULATION_STAR.
@@ -479,25 +541,26 @@ Section INJ_SIMULATION_PLUS.
   Variable measure: C1 -> nat. 
   Hypothesis inj_plus_simulation:
     forall c1 m1 c1' m1', corestep Sem1 ge1 c1 m1 c1' m1'  -> 
-    forall c2 r m2 j, match_states c1 r j c1 m1 c2 m2 ->
-      exists c2', exists m2', exists r', exists j', 
-        inject_incr j j' /\
-        inject_separated j j' m1 m2 /\ 
-        reserve_map_incr r r' /\
-        reserve_map_separated r r' j' m1 m2 /\ 
-        mem_unchanged_on (guarantee_left Sem1 r c1) m1 m1' /\
-        mem_unchanged_on (guarantee_right Sem1 j r c1) m2 m2' /\
-        match_states c1' r' j' c1' m1' c2' m2' /\
-        corestep_plus Sem2 ge2 c2 m2 c2' m2'.
+      forall c2 (r: reserve) m2 j, 
+        guarantee Sem1 r c1' m1' /\
+        match_states c1 r j c1 m1 c2 m2 ->
+        exists c2', exists m2', exists r', exists j', 
+          inject_incr j j' /\
+          inject_separated j j' m1 m2 /\ 
+          reserve_incr r r' /\
+          reserve_separated r r' j' m1 m2 /\ 
+          guarantee' Sem2 j r c2' m2' /\
+          match_states c1' r' j' c1' m1' c2' m2' /\
+          corestep_plus Sem2 ge2 c2 m2 c2' m2'.
   
 Lemma inj_simulation_plus: 
   Forward_simulation_inj.Forward_simulation_inject _ _ Sem1 Sem2 ge1 ge2 entry_points.
 Proof.
   apply inj_simulation_star with (measure:=measure).
   intros. exploit inj_plus_simulation; eauto.
-  intros [? [? [? [? [? [? [? [? [? [? [? ?]]]]]]]]]]].
+  intros [? [? [? [? [? [? [? [? [? [? ?]]]]]]]]]].
   do 4 eexists. split; eauto. split; eauto.
-   split; eauto. solve[split; eauto].
+  solve[split; eauto]. 
 Qed.
 
 End INJ_SIMULATION_PLUS.
